tuned

thys/Amortized_Complexity/Pairing_Heap2.thy
@@ -29,7 +29,7 @@ fun pass\<^sub>1 :: "'a :: linorder tree \<Rightarrow> 'a tree" where
 
 fun len :: "'a tree \<Rightarrow> nat" where 
   "len Leaf = 0"
-| "len (Node _ _ r) = 1 + len r"
+| "len (Node _ _ r) = len r + 1"
 
 fun pass\<^sub>2 :: "'a :: linorder tree \<Rightarrow> 'a tree" where
   "pass\<^sub>2 Leaf = Leaf"
@@ -38,7 +38,8 @@ fun pass\<^sub>2 :: "'a :: linorder tree \<Rightarrow> 'a tree" where
 fun mergepairs :: "'a :: linorder tree \<Rightarrow> 'a tree" where
   "mergepairs Leaf = Leaf"
 | "mergepairs (Node lx x Leaf) = Node lx x Leaf" 
-| "mergepairs (Node lx x (Node ly y ry)) = link (link (Node lx x (Node ly y (mergepairs ry))))"
+| "mergepairs (Node lx x (Node ly y ry)) =
+   link (link (Node lx x (Node ly y (mergepairs ry))))"
 
 fun del_min :: "'a :: linorder tree \<Rightarrow> 'a tree" where
   "del_min Leaf = Leaf"
@@ -52,24 +53,24 @@ fun meld :: "'a :: linorder tree \<Rightarrow> 'a tree \<Rightarrow> 'a tree" wh
 fun insert :: "'a \<Rightarrow> 'a :: linorder tree \<Rightarrow> 'a tree" where
   "insert x h = meld (Node Leaf x Leaf) h"
 
-fun isRoot :: "'a :: linorder tree \<Rightarrow> bool" where
-  "isRoot h = (case h of Leaf \<Rightarrow> True | Node l x r \<Rightarrow> r = Leaf)"
+fun is_root :: "'a :: linorder tree \<Rightarrow> bool" where
+  "is_root h = (case h of Leaf \<Rightarrow> True | Node l x r \<Rightarrow> r = Leaf)"
 
 fun \<Phi> :: "'a tree \<Rightarrow> real" where
   "\<Phi> Leaf = 0"
-| "\<Phi> (Node l _ r) = \<Phi> l + \<Phi> r + log 2 (1 + size l + size r)"
+| "\<Phi> (Node l _ r) = \<Phi> l + \<Phi> r + log 2 (size l + size r + 1)"
 
-lemma link_size[simp]: "size (link h) = size h" 
-  by (cases h rule: link.cases) simp_all
+lemma link_size[simp]: "size (link hs) = size hs" 
+  by (cases hs rule: link.cases) simp_all
 
-lemma size_pass\<^sub>1: "size (pass\<^sub>1 h) = size h" 
-  by (induct h rule: pass\<^sub>1.induct) simp_all
+lemma size_pass\<^sub>1: "size (pass\<^sub>1 hs) = size hs" 
+  by (induct hs rule: pass\<^sub>1.induct) simp_all
 
-lemma size_pass\<^sub>2: "size (pass\<^sub>2 h) = size h" 
-  by (induct h rule: pass\<^sub>2.induct) simp_all
+lemma size_pass\<^sub>2: "size (pass\<^sub>2 hs) = size hs" 
+  by (induct hs rule: pass\<^sub>2.induct) simp_all
 
 lemma size_meld[simp]: 
-  "isRoot h1 \<Longrightarrow> isRoot h2 \<Longrightarrow> size (meld h1 h2) = size h1 + size h2"
+  "is_root h1 \<Longrightarrow> is_root h2 \<Longrightarrow> size (meld h1 h2) = size h1 + size h2"
   by (simp split: tree.splits)
 
 lemma link_struct: "\<exists>la a. link (Node lx x (Node ly y ry)) = Node la a ry" 
@@ -82,37 +83,37 @@ lemma pass\<^sub>2_struct: "\<exists>la a. pass\<^sub>2 (Node lx x rx) = Node la
   by (induction rx arbitrary: x lx rule: pass\<^sub>2.induct) 
   (simp, metis pass\<^sub>2.simps(2) link_struct)
 
-lemma mergepairs_pass12: "mergepairs h = pass\<^sub>2 (pass\<^sub>1 h)"
-by (induction h rule: mergepairs.induct) auto
+lemma mergepairs_pass12: "mergepairs hs = pass\<^sub>2 (pass\<^sub>1 hs)"
+by (induction hs rule: mergepairs.induct) auto
 
-lemma \<Delta>\<Phi>_insert: "isRoot h \<Longrightarrow> \<Phi> (insert x h) - \<Phi> h \<le> log 2  (size h + 1)"
+lemma \<Delta>\<Phi>_insert: "is_root h \<Longrightarrow> \<Phi> (insert x h) - \<Phi> h \<le> log 2  (size h + 1)"
   by (simp split: tree.splits)
 
 lemma \<Delta>\<Phi>_meld:
   assumes "h1 = Node lx x Leaf" "h2 = Node ly y Leaf" 
   shows "\<Phi> (meld h1 h2) - \<Phi> h1 - \<Phi> h2 \<le> 2*log 2 (size h1 + size h2)" 
 proof -
-  let ?h = "Node lx x (Node ly y Leaf)"
-  have "\<Phi> (link ?h) - \<Phi> ?h \<le> log 2  (1 + size lx + size ly)" by (simp add: algebra_simps)
+  let ?hs = "Node lx x (Node ly y Leaf)"
+  have "\<Phi> (link ?hs) - \<Phi> ?hs \<le> log 2  (size lx + size ly + 1)" by (simp add: algebra_simps)
   also have "\<dots> \<le> log 2  (size h1 + size h2)" by (simp add: assms)
-  moreover have "\<Phi> ?h - \<Phi> h1 - \<Phi> h2 \<le> \<dots>" using assms by simp
-  ultimately have "\<Phi> (link ?h) - \<Phi> h1 - \<Phi> h2 \<le> 2*\<dots>" by linarith
+  moreover have "\<Phi> ?hs - \<Phi> h1 - \<Phi> h2 \<le> \<dots>" using assms by simp
+  ultimately have "\<Phi> (link ?hs) - \<Phi> h1 - \<Phi> h2 \<le> 2*\<dots>" by linarith
   thus ?thesis using assms by simp
 qed
 
 fun upperbound :: "'a tree \<Rightarrow> real" where
   "upperbound Leaf = 0"
 | "upperbound (Node _ _ Leaf) = 0"
-| "upperbound (Node lx _ (Node ly _ Leaf)) = 2*log 2 (2 + size lx + size ly)" 
-| "upperbound (Node lx _ (Node ly _ ry)) = 2*log 2 (2 + size lx + size ly + size ry) 
+| "upperbound (Node lx _ (Node ly _ Leaf)) = 2*log 2 (size lx + size ly + 2)" 
+| "upperbound (Node lx _ (Node ly _ ry)) = 2*log 2 (size lx + size ly + size ry + 2) 
     - 2*log 2 (size ry) - 2 + upperbound ry"
 
-lemma \<Delta>\<Phi>_pass1_upperbound: "\<Phi> (pass\<^sub>1 h) - \<Phi> h  \<le> upperbound h"
-proof (induction h rule: upperbound.induct)
+lemma \<Delta>\<Phi>_pass1_upperbound: "\<Phi> (pass\<^sub>1 hs) - \<Phi> hs  \<le> upperbound hs"
+proof (induction hs rule: upperbound.induct)
   case (3 lx x ly y)
-  have "log 2  (1 + size lx + size ly) - log 2  (1 + size ly) 
-    \<le> log 2 (1 + size lx + size ly)" by simp
-  also have "\<dots> \<le> log 2 (2 + size lx + size ly)" by simp
+  have "log 2  (size lx + size ly + 1) - log 2  (size ly + 1) 
+    \<le> log 2 (size lx + size ly + 1)" by simp
+  also have "\<dots> \<le> log 2 (size lx + size ly + 2)" by simp
   also have "\<dots> \<le> 2*\<dots>" by simp
   finally show ?case by (simp add: algebra_simps)
 next
@@ -120,13 +121,13 @@ next
   let ?ry = "Node lz z rz"
   let ?rx = "Node ly y ?ry"
   let ?h = "Node lx x ?rx"
-  let ?t ="log 2 (1 + size lx + size ly) - log 2 (1 + size ly + size ?ry)"
+  let ?t ="log 2 (size lx + size ly + 1) - log 2 (size ly + size ?ry + 1)"
   have "\<Phi> (pass\<^sub>1 ?h) - \<Phi> ?h \<le> ?t + upperbound ?ry" 
     using "4.IH" by (simp add: size_pass\<^sub>1 algebra_simps)
   also have "?t \<le> 2*log 2  (size ?h) - 2*log 2 (size ?ry) - 2"
   proof -
-    have "log 2  (1 + size lx + size ly) + log 2  (size ?ry) - 2*log 2  (size ?h) 
-      = log 2 ((1 + size lx + size ly)/(size ?h) ) + log 2 (size ?ry / size ?h)"
+    have "log 2 (size lx + size ly + 1) + log 2  (size ?ry) - 2*log 2 (size ?h) 
+      = log 2 ((size lx + size ly + 1)/(size ?h) ) + log 2 (size ?ry / size ?h)"
       (is "_ = log 2 ?t1 + log 2 ?t2") by (simp add: log_divide)
     also have "\<dots> \<le> -2" 
     proof -
@@ -135,50 +136,51 @@ next
       also have "\<dots> \<le> 0" by (simp add: field_simps del: of_nat_Suc)
       finally show ?thesis by linarith
     qed 
-    finally have "log 2 (1 + size lx + size ly) + log 2 (size ?ry) + 2
+    finally have "log 2 (size lx + size ly + 1) + log 2 (size ?ry) + 2
       \<le>  2*log 2 (size ?h)" by simp
     moreover have "log 2 (size ?ry) \<le> log 2 (size ?rx)" by simp  
-    ultimately have "log 2 (1 + size lx + size ly) - \<dots> 
+    ultimately have "log 2 (size lx + size ly + 1) - \<dots> 
       \<le>  2*log 2 (size ?h) - 2*log 2 (size ?ry) - 2" by linarith
     thus ?thesis by simp
   qed
   finally show ?case by (simp add: algebra_simps)
 qed simp_all
 
-lemma \<Delta>\<Phi>_pass1: assumes "h \<noteq> Leaf"
-  shows "\<Phi> (pass\<^sub>1 h) - \<Phi> h \<le> 2*log 2 (size h) - len h + 2"
+lemma \<Delta>\<Phi>_pass1: assumes "hs \<noteq> Leaf"
+  shows "\<Phi> (pass\<^sub>1 hs) - \<Phi> hs \<le> 2*log 2 (size hs) - len hs + 2"
 proof -
-  have "h \<noteq> Leaf \<Longrightarrow> upperbound h \<le> 2*log 2 (size h) - len h + 2" 
-    by (induct h rule: upperbound.induct) (simp_all add: algebra_simps)
-  thus ?thesis using assms \<Delta>\<Phi>_pass1_upperbound [of "h"] order_trans by blast
+  from assms have "upperbound hs \<le> 2*log 2 (size hs) - len hs + 2" 
+    by (induct hs rule: upperbound.induct) (simp_all add: algebra_simps)
+  thus ?thesis using \<Delta>\<Phi>_pass1_upperbound [of "hs"] order_trans by blast
 qed
 
-lemma \<Delta>\<Phi>_pass2: "h \<noteq> Leaf \<Longrightarrow> \<Phi> (pass\<^sub>2 h) - \<Phi> h \<le> log 2 (size h)"
-proof (induction h rule: pass\<^sub>2.induct)
+lemma \<Delta>\<Phi>_pass2: "hs \<noteq> Leaf \<Longrightarrow> \<Phi> (pass\<^sub>2 hs) - \<Phi> hs \<le> log 2 (size hs)"
+proof (induction hs rule: pass\<^sub>2.induct)
   case (2 lx x rx)
   thus ?case 
   proof (cases rx)
-    case [simp]: (Node ly y ry)
+    case *: (Node ly y ry)
     let ?h = "Node lx x rx"
-    obtain la a where 1: "pass\<^sub>2 rx = Node la a Leaf" 
-      using pass\<^sub>2_struct by force
+    obtain la a where **: "pass\<^sub>2 rx = Node la a Leaf" 
+      using pass\<^sub>2_struct * by force
     hence "size \<dots> = size rx" using size_pass\<^sub>2 by metis
     hence "\<Phi> (pass\<^sub>2 ?h) - \<Phi> ?h  
       \<le> log 2 (size ?h) - log 2  \<dots> + \<Phi> (pass\<^sub>2 rx) - \<Phi> rx"
-      using 1 by (simp add: algebra_simps) 
-    thus ?thesis using "2.IH" 1 by simp
+      using * ** by (simp add: algebra_simps) 
+    thus ?thesis using "2.IH" * by simp
   qed simp
 qed simp
 
-lemma \<Delta>\<Phi>_mergepairs: assumes "h \<noteq> Leaf"
-  shows "\<Phi> (mergepairs h) - \<Phi> h \<le> 3 * log 2 (size h) - len h + 2"
+lemma \<Delta>\<Phi>_mergepairs: assumes "hs \<noteq> Leaf"
+  shows "\<Phi> (mergepairs hs) - \<Phi> hs \<le> 3 * log 2 (size hs) - len hs + 2"
 proof -
-  have "pass\<^sub>1 h \<noteq> Leaf" by (metis assms size_0_iff_Leaf size_pass\<^sub>1)
-  with assms \<Delta>\<Phi>_pass1[of h] \<Delta>\<Phi>_pass2[of "pass\<^sub>1 h"]
+  have "pass\<^sub>1 hs \<noteq> Leaf" by (metis assms size_0_iff_Leaf size_pass\<^sub>1)
+  with assms \<Delta>\<Phi>_pass1[of hs] \<Delta>\<Phi>_pass2[of "pass\<^sub>1 hs"]
   show ?thesis by (auto simp add: size_pass\<^sub>1 mergepairs_pass12)
 qed
 
-lemma \<Delta>\<Phi>_del_min:  "lx \<noteq> Leaf \<Longrightarrow> \<Phi> (del_min (Node lx x Leaf)) - \<Phi> (Node lx x Leaf) 
+lemma \<Delta>\<Phi>_del_min: "lx \<noteq> Leaf \<Longrightarrow>
+  \<Phi> (del_min (Node lx x Leaf)) - \<Phi> (Node lx x Leaf) 
   \<le> 3*log 2 (size lx) - len lx + 2"
 proof -
   let ?h = "Node lx x Leaf"
@@ -195,13 +197,15 @@ proof -
   ultimately show ?thesis by linarith
 qed
 
-lemma isRoot_meld: "isRoot h1 \<Longrightarrow> isRoot h2 \<Longrightarrow> isRoot (meld h1 h2)"
-  by (simp split: tree.splits)
+lemma is_root_meld:
+  "is_root h1 \<Longrightarrow> is_root h2 \<Longrightarrow> is_root (meld h1 h2)"
+by (simp split: tree.splits)
 
-lemma isRoot_insert: "isRoot h \<Longrightarrow> isRoot (insert x h)"
-  by (simp split: tree.splits)
+lemma is_root_insert: "is_root h \<Longrightarrow> is_root (insert x h)"
+by (simp split: tree.splits)
 
-lemma isRoot_del_min: assumes "isRoot h" shows "isRoot (del_min h)"
+lemma is_root_del_min:
+  assumes "is_root h" shows "is_root (del_min h)"
 proof (cases h)
   case [simp]: (Node lx x rx)
   have "rx = Leaf" using assms by simp
@@ -217,7 +221,7 @@ proof (cases h)
 qed simp
 
 lemma pass\<^sub>1_len: "len (pass\<^sub>1 h) \<le> len h"
-  by (induct h rule: pass\<^sub>1.induct) simp_all
+by (induct h rule: pass\<^sub>1.induct) simp_all
 
 fun exec :: "'a :: linorder op\<^sub>p\<^sub>q \<Rightarrow> 'a tree list \<Rightarrow> 'a tree" where
 "exec Empty [] = Leaf" | 
@@ -228,30 +232,30 @@ fun exec :: "'a :: linorder op\<^sub>p\<^sub>q \<Rightarrow> 'a tree list \<Righ
 fun t\<^sub>p\<^sub>a\<^sub>s\<^sub>s\<^sub>1 :: "'a tree \<Rightarrow> nat" where
   "t\<^sub>p\<^sub>a\<^sub>s\<^sub>s\<^sub>1 Leaf = 1"
 | "t\<^sub>p\<^sub>a\<^sub>s\<^sub>s\<^sub>1 (Node _ _ Leaf) = 1"
-| "t\<^sub>p\<^sub>a\<^sub>s\<^sub>s\<^sub>1 (Node _ _ (Node _ _ ry)) = 1 + t\<^sub>p\<^sub>a\<^sub>s\<^sub>s\<^sub>1 ry"
+| "t\<^sub>p\<^sub>a\<^sub>s\<^sub>s\<^sub>1 (Node _ _ (Node _ _ ry)) = t\<^sub>p\<^sub>a\<^sub>s\<^sub>s\<^sub>1 ry + 1"
 
 fun t\<^sub>p\<^sub>a\<^sub>s\<^sub>s\<^sub>2 :: "'a tree \<Rightarrow> nat" where
   "t\<^sub>p\<^sub>a\<^sub>s\<^sub>s\<^sub>2 Leaf = 1"
-| "t\<^sub>p\<^sub>a\<^sub>s\<^sub>s\<^sub>2 (Node _ _ rx) = 1 + t\<^sub>p\<^sub>a\<^sub>s\<^sub>s\<^sub>2 rx"
+| "t\<^sub>p\<^sub>a\<^sub>s\<^sub>s\<^sub>2 (Node _ _ rx) = t\<^sub>p\<^sub>a\<^sub>s\<^sub>s\<^sub>2 rx + 1"
 
 fun cost :: "'a :: linorder op\<^sub>p\<^sub>q \<Rightarrow> 'a tree list \<Rightarrow> nat" where
   "cost Empty [] = 1"
 | "cost Del_min [Leaf] = 1"
-| "cost Del_min [Node lx _  _] = 1 + t\<^sub>p\<^sub>a\<^sub>s\<^sub>s\<^sub>2 (pass\<^sub>1 lx) + t\<^sub>p\<^sub>a\<^sub>s\<^sub>s\<^sub>1 lx"
+| "cost Del_min [Node lx _  _] = t\<^sub>p\<^sub>a\<^sub>s\<^sub>s\<^sub>2 (pass\<^sub>1 lx) + t\<^sub>p\<^sub>a\<^sub>s\<^sub>s\<^sub>1 lx + 1"
 | "cost (Insert a) _ = 1"
-| "cost Meld [h1,h2] = 1"
+| "cost Meld _ = 1"
 
 fun U :: "'a :: linorder op\<^sub>p\<^sub>q \<Rightarrow> 'a tree list \<Rightarrow> real" where
   "U Empty [] = 1"
-| "U (Insert a) [h] = log 2 (1 + size h) + 1"
-| "U Del_min [h] = 3*log 2 (1 + size h) + 5"
-| "U Meld [h1,h2] = 2*log 2 (1 + size h1 + size h2) + 1"
+| "U (Insert a) [h] = log 2 (size h + 1) + 1"
+| "U Del_min [h] = 3*log 2 (size h + 1) + 5"
+| "U Meld [h1,h2] = 2*log 2 (size h1 + size h2 + 1) + 1"
 
 interpretation Amortized
-where arity = arity and exec = exec and cost = cost and inv = isRoot 
+where arity = arity and exec = exec and cost = cost and inv = is_root 
 and \<Phi> = \<Phi> and U = U
 proof
-  case goal1 thus ?case using isRoot_insert isRoot_del_min isRoot_meld
+  case goal1 thus ?case using is_root_insert is_root_del_min is_root_meld
     by (cases f) (auto simp: numeral_eq_Suc)
 next
   case goal2 show ?case by (induct s) simp_all
@@ -263,7 +267,7 @@ next
     case Empty with goal4 show ?thesis by(auto)
   next
     case (Insert x)
-    then obtain h where "ss = [h]" "isRoot h" using goal4 by auto
+    then obtain h where "ss = [h]" "is_root h" using goal4 by auto
     thus ?thesis using Insert \<Delta>\<Phi>_insert goal4 by auto
   next
     case [simp]: (Del_min)
@@ -274,19 +278,19 @@ next
       have "t\<^sub>p\<^sub>a\<^sub>s\<^sub>s\<^sub>2 (pass\<^sub>1 lx) + t\<^sub>p\<^sub>a\<^sub>s\<^sub>s\<^sub>1 lx \<le> len lx + 2"
         by (induct lx rule: pass\<^sub>1.induct) simp_all
       hence "cost f ss \<le> \<dots> + 1" by simp 
-      moreover have "\<Phi> (del_min h) - \<Phi> h \<le> 3*log 2 (1 + size h) - len lx + 2"
+      moreover have "\<Phi> (del_min h) - \<Phi> h \<le> 3*log 2 (size h + 1) - len lx + 2"
       proof (cases lx)
         case [simp]: (Node ly y ry) 
         have "\<Phi> (del_min h) - \<Phi> h \<le> 3*log 2 (size lx) - len lx + 2"
           using  \<Delta>\<Phi>_del_min[of "lx" "x"] goal4 by simp
-        also have "\<dots> \<le> 3*log 2 (1 + size h) - len lx + 2" by fastforce
+        also have "\<dots> \<le> 3*log 2 (size h + 1) - len lx + 2" by fastforce
         finally show ?thesis by blast
       qed (insert goal4, simp)
       ultimately show ?thesis by auto
     qed simp
   next
     case [simp]: Meld
-    then obtain h1 h2 where [simp]: "ss = [h1,h2]" and 1: "isRoot h1" "isRoot h2"
+    then obtain h1 h2 where [simp]: "ss = [h1,h2]" and 1: "is_root h1" "is_root h2"
       using goal4 by (auto simp: numeral_eq_Suc)
     show ?thesis
     proof (cases h1)
@@ -300,7 +304,7 @@ next
         case h2: Node
         have "\<Phi> (meld h1 h2) - \<Phi> h1 - \<Phi> h2 \<le> 2 * log 2 (real (size h1 + size h2))"
           apply(rule \<Delta>\<Phi>_meld) using h1 h2 1 by auto
-        also have "\<dots> \<le> 2 * log 2 (1 + size h1 + size h2)" by (simp add: h1)
+        also have "\<dots> \<le> 2 * log 2 (size h1 + size h2 + 1)" by (simp add: h1)
         finally show ?thesis by(simp)
       qed
     qed
